src/tls/Crypto.AE.fsti
@@ -20,7 +20,7 @@ val encrypt
   (plain: plain_p a)
   (plain_len: U32.t {U32.v plain_len == B.length plain})
   (cipher: cipher_p a) // cipher == iv ++ cipher ++ tag (see EverCrypt.AEAD.encrypt_st)
-: HST.Stack EE.error_code
+: HST.Stack unit
   (requires (fun h ->
     invariant h s /\
     B.live h plain /\
@@ -31,17 +31,12 @@ val encrypt
     B.disjoint plain cipher /\
     B.length cipher == B.length plain + iv_length + SC.tag_length a
   ))
-  (ensures (fun h res h' -> 
-    match res with
-    | EE.InvalidKey ->
-      B.modifies (B.loc_buffer cipher) h h' // TODO: should be False, need to fix EverCrypt
-    | EE.Success ->
+  (ensures (fun h _ h' ->
       let iv = B.gsub cipher 0ul iv_len in
       let cipher' = B.gsub cipher iv_len (B.len cipher `U32.sub` iv_len) in
       B.modifies (B.loc_union (footprint s) (B.loc_buffer cipher)) h h' /\
       invariant h' s /\
       (F.ideal_AEAD == false ==> SC.encrypt (state_kv s) (Cast.to_seq_sec8 (B.as_seq h' iv)) Seq.empty (Cast.to_seq_sec8 (B.as_seq h plain)) `Seq.equal` Cast.to_seq_sec8 (B.as_seq h' cipher'))
-    | _ -> False
   ))
 
 // decrypt is unchanged from Crypto.AEAD.decrypt
